src/coq/Effects.v
@@ -61,11 +61,11 @@ Defined.
 
 (* Domain of semantics *)
 CoInductive D X :=
-| Ret : X -> D X
-| Fin : value -> D X
-| Err : string -> D X 
-| Tau : D X -> D X
-| Eff : effects (D X) -> D X 
+| Ret : X -> D X        (* Unfinished trace *)
+| Fin : value -> D X    (* Finished trace *) 
+| Err : string -> D X   (* Abort with an error *)
+| Tau : D X -> D X      (* Internal step of computation *)
+| Eff : effects (D X) -> D X    (* Externally visible step of computation *)
 .
 
 CoFixpoint d_map {A B} (f:A -> B) (d:D A) : D B :=
@@ -99,6 +99,37 @@ End UNFOLDING.
 Arguments id_d_eq {_} _ .
 
 
+(* Error predicate, which says whether an observation trace leads to an error allong *)
+Inductive d_error_free_mem_step {A} (R: D A -> Prop) : effects (D A) -> Prop :=
+| d_error_free_mem_Alloca : forall t f, (forall (a:addr), R (f (inj_addr a))) -> d_error_free_mem_step R (Alloca t f)
+| d_error_free_mem_Load   : forall a f, (forall (dv:value), R (f dv)) -> d_error_free_mem_step R (Load a f)
+| d_error_free_mem_Store  : forall a n d, R d -> d_error_free_mem_step R (Store a n d)
+| d_error_free_mem_Call   : forall v f, (forall (dv:value), R (f dv)) -> d_error_free_mem_step R (Call v f)
+.                                                                                
+
+(* No cases for Ret or Err --
+   Ret means an "unfinished" computation (and shouldn't arise in the semantics of a CFG program)
+   Err definitely has an error, which this predicate rules out
+*)
+Inductive d_error_free_step {A} (R: D A -> Prop) : D A -> Prop :=
+| d_error_free_step_fin : forall v, d_error_free_step R (Fin v)
+| d_error_free_step_tau : forall d, R d -> d_error_free_step R (Tau d)
+| d_error_free_step_eff : forall m, d_error_free_mem_step R m -> d_error_free_step R (Eff m)
+.                                                                             
+Hint Constructors d_error_free_mem_step d_error_free_step.
+
+Definition d_error_free {A} := paco1 (@d_error_free_step A) bot1.
+Hint Unfold d_error_free.
+
+Lemma d_error_free_gen_mon {A} : monotone1 (@d_error_free_step A).
+Proof.
+  unfold monotone1. intros.
+  induction IN; eauto.
+  eapply d_error_free_step_eff.
+  induction H; constructor; auto.
+Qed.
+Hint Resolve d_error_free_gen_mon : paco.
+
 (*
   This relation doesn't allow any variation in the relations for the memory model.  A more parametric version would:
     - have an address relation  A : addr -> addr -> Prop  
@@ -123,36 +154,7 @@ Inductive d_equiv_step {A} (R:D A -> D A -> Prop) : D A -> D A -> Prop :=
 
 Hint Constructors d_equiv_mem_step d_equiv_step.  (* d_equiv *)
 
-Definition d_equiv {A} (p q : D A) := paco2 (@d_equiv_step A) bot2 p q.
-Hint Unfold d_equiv.
-
-Instance D_functor : @Functor D := fun A => fun B => @d_map A B.
-
-(* Probably a functor only up to stuttering equivalence. *)
-(*
-Program Instance D_functor_eq_laws : (@FunctorLaws D) D_functor (@eq).
-*)
-
-(* Note: for guardedness, bind Ret introduces extra Tau *)
-Definition bind {A B} (m:D A) (f:A -> D B) : D B :=
-  (cofix bindf m:= 
-     match m with
-       | Ret a => Tau (f a)
-       | Fin d => Fin d
-       | Err s => Err s
-       | Tau d' => Tau (bindf d')
-       | Eff m => Eff (effects_map bindf m)
-     end) m.
-
-Program Instance D_monad : (@Monad D) (@D_functor) := _.
-Next Obligation.
-  split.
-  - intros. apply Ret. exact X.
-  - intros A B. apply bind.
-Defined.
-
 Lemma d_equiv_gen_mon A : monotone2 (@d_equiv_step A).
-  pmonauto.
 Proof.
   unfold monotone2. intros. induction IN; eauto.
   eapply d_equiv_step_eff. induction H.
@@ -161,8 +163,237 @@ Proof.
   - constructor. eauto.
   - constructor. eauto.
 Qed.
-
 Hint Resolve d_equiv_gen_mon : paco.
+
+Definition d_equiv {A} (p q : D A) := paco2 (@d_equiv_step A) bot2 p q.
+Hint Unfold d_equiv.
+
+
+Inductive d_equiv_step' {A} (R:D A -> D A -> Prop) : D A -> D A -> Prop :=
+| d_equiv_step'_ret : forall a, d_equiv_step' R (Ret a) (Ret a)
+| d_equiv_step'_fin : forall v, d_equiv_step' R (Fin v) (Fin v)
+| d_equiv_step'_err : forall s1 s2, d_equiv_step' R (Err s1) (Err s2)
+| d_equiv_step'_tau : forall d1 d2, R d1 d2 -> d_equiv_step' R (Tau d1) (Tau d2)
+| d_equiv_step'_lft : forall d1 d2, R d1 d2 -> d_equiv_step' R (Tau d1) d2
+| d_equiv_step'_rgt : forall d1 d2, R d1 d2 -> d_equiv_step' R d1 (Tau d2)
+| d_equiv_step'_eff : forall m1 m2, d_equiv_mem_step R m1 m2 -> d_equiv_step' R (Eff m1) (Eff m2)
+.    
+
+Hint Constructors d_equiv_step'.
+Lemma d_equiv_gen_mon' A : monotone2 (@d_equiv_step' A).
+Proof.
+  unfold monotone2. intros. induction IN; eauto.
+  eapply d_equiv_step'_eff. induction H.
+  - constructor. eauto.
+  - constructor. eauto.
+  - constructor. eauto.
+  - constructor. eauto.
+Qed.
+Hint Resolve d_equiv_gen_mon' : paco.
+
+Definition d_equiv' {A} (p q : D A) := paco2 (@d_equiv_step' A) bot2 p q.
+Hint Unfold d_equiv'.
+
+Lemma d_equivalent : forall A (p q : D A), d_equiv p q -> d_equiv' p q.
+Proof.
+  intros A. 
+  pcofix CIH. intros p q H.
+  pfold.
+  punfold H. remember (upaco2 d_equiv_step bot2).
+  induction H; subst; eauto.
+  - apply d_equiv_step'_tau. right. apply CIH. inversion H. apply H0. inversion H0.
+  - apply d_equiv_step'_eff. remember (upaco2 d_equiv_step bot2).
+    induction H.
+    + constructor. intros. right. apply CIH. subst. specialize (H a). destruct H. exact H. inversion H.
+    + constructor. intros. right. apply CIH. subst. specialize (H dv). destruct H. exact H. inversion H.
+    + constructor. intros. right. apply CIH. subst. destruct H. exact H. inversion H.      
+    + constructor. intros. right. apply CIH. subst. specialize (H dv). destruct H. exact H. inversion H.      
+Qed.
+
+Fixpoint taus {A} (n:nat) (d:D A) : D A :=
+  match n with
+  | 0 => d
+  | S n => Tau (taus n d)
+  end.
+
+Lemma d_equivalent' : forall A (p q : D A), d_equiv' p q -> d_equiv p q.
+Proof.
+  intros A.
+  pcofix CIH. intros p q H.
+  pfold.  
+  punfold H. simpl. remember (upaco2 d_equiv_step' bot2).
+  destruct H; subst; eauto.
+  + constructor. right. apply CIH. destruct H. exact H. inversion H.
+  + constructor. destruct H. destruct H. destruct SIM; subst; eauto.
+      * constructor. apply LE in H. right. apply CIH. destruct H. exact H. inversion H.
+      * constructor. apply LE in H. destruct H. apply CIH in H. 
+    
+
+    
+        
+
+
+
+
+
+
+
+
+
+
+
+
+
+
+
+
+
+
+
+
+
+
+
+
+
+
+
+
+
+
+
+
+
+
+
+
+
+
+
+
+
+
+
+
+
+
+
+
+
+
+
+
+
+
+
+
+
+
+
+
+
+
+
+
+
+
+
+
+
+
+
+
+
+
+
+
+
+
+
+
+
+
+
+
+
+
+
+
+
+
+      
+
+
+Instance D_functor : @Functor D := fun A => fun B => @d_map A B.
+
+
+
+(* Probably a functor only up to stuttering equivalence. *)
+(*
+Program Instance D_functor_eq_laws : (@FunctorLaws D) D_functor (@eq).
+*)
+Lemma d_equiv_refl : forall {A} (d : D A), d_equiv d d.
+Proof.
+  intro. pcofix CIH.
+  intros. pfold. destruct d; eauto.
+  destruct e; eauto. 
+Qed.
+
+Lemma d_equiv_symm : forall {A} (d1 d2 : D A), d_equiv d1 d2 -> d_equiv d2 d1.
+Proof.
+  intro. pcofix CIH.
+  intros d1 d2 H.
+  punfold H. remember (upaco2 d_equiv_step bot2).
+  induction H; eauto; subst.
+  - pfold. constructor. right. eapply CIH.
+    destruct H; eauto. inversion H. 
+  - pfold. constructor. punfold IHd_equiv_step.
+  - pfold. constructor. punfold IHd_equiv_step.
+  - pfold. constructor. inversion H; subst.
+    + constructor. intro. specialize (H0 a). destruct H0.
+      right. eapply CIH. eapply H0. inversion H0.
+    + constructor. intro. specialize (H0 dv). destruct H0.
+      right. eapply CIH. eapply H0. inversion H0.
+    + constructor. right. eapply CIH. destruct H0; eauto. inversion H0. 
+    + constructor. intro. specialize (H0 dv). destruct H0.
+      right. eapply CIH. eapply H0. inversion H0.
+Qed.
+
+(* Note: for guardedness, bind Ret introduces extra Tau *)
+Definition bind {A B} (f:A -> D B) : D A -> D B :=
+  (cofix bindf := fun m => 
+     match m with
+       | Ret a => Tau (f a)
+       | Fin d => Fin d
+       | Err s => Err s
+       | Tau d' => Tau (bindf d')
+       | Eff m => Eff (effects_map bindf m)
+     end).
+
+Lemma bind_unfold : forall {A B} (m:D A) (f:A -> D B),
+    d_equiv (bind f m)
+    (match m with
+    | Ret a => Tau (f a)
+    | Fin d => Fin d
+    | Err s => Err s
+    | Tau d' => Tau (bind f d')
+    | Eff e => Eff (effects_map (bind f) e)
+    end).
+Proof.
+  intros A B.
+  pcofix CIH. intros m f.
+  pfold. rewrite (id_d_eq (bind f m)). simpl.
+  destruct m; simpl; auto. apply d_equiv_step_tau. right.
+  
+  
+  
+
+Program Instance D_monad : (@Monad D) (@D_functor) := _.
+Next Obligation.
+  split.
+  - intros. apply Ret. exact X.
+  - intros A B. apply bind.
+Defined.
 
 
 Ltac punfold' H := let x := fresh "_x_" in
@@ -205,11 +436,6 @@ Section D_EQUIV_COIND.
 End D_EQUIV_COIND.
 Arguments d_equiv_coind [_] _ [_ _] _ _.
 
-Fixpoint taus {A} (n:nat) (d:D A) : D A :=
-  match n with
-  | 0 => d
-  | S n => Tau (taus n d)
-  end.
 
 Lemma stutter_helper : forall {A} (d1 d2 : D A), d_equiv (Tau d1) d2 -> d_equiv d1 d2.
 Proof.
@@ -228,32 +454,6 @@ Proof.
   eapply IHn. simpl in H. eapply stutter_helper. eapply H.
 Qed.
 
-Lemma d_equiv_refl : forall {A} (d : D A), d_equiv d d.
-Proof.
-  intro. pcofix CIH.
-  intros. pfold. destruct d; eauto.
-  destruct e; eauto. 
-Qed.
-
-Lemma d_equiv_symm : forall {A} (d1 d2 : D A), d_equiv d1 d2 -> d_equiv d2 d1.
-Proof.
-  intro. pcofix CIH.
-  intros d1 d2 H.
-  punfold H. remember (upaco2 d_equiv_step bot2).
-  induction H; eauto; subst.
-  - pfold. constructor. right. eapply CIH.
-    destruct H; eauto. inversion H. 
-  - pfold. constructor. punfold IHd_equiv_step.
-  - pfold. constructor. punfold IHd_equiv_step.
-  - pfold. constructor. inversion H; subst.
-    + constructor. intro. specialize (H0 a). destruct H0.
-      right. eapply CIH. eapply H0. inversion H0.
-    + constructor. intro. specialize (H0 dv). destruct H0.
-      right. eapply CIH. eapply H0. inversion H0.
-    + constructor. right. eapply CIH. destruct H0; eauto. inversion H0. 
-    + constructor. intro. specialize (H0 dv). destruct H0.
-      right. eapply CIH. eapply H0. inversion H0.
-Qed.
 
 Lemma stutter : forall {A} (d1 d2 : D A) n m, d_equiv (taus n d1) (taus m d2) -> d_equiv d1 d2.
 Proof.
